Missing invariant, with a comment

experiments/Veritas.VCache.fst
@@ -31,6 +31,8 @@ let as_seq st h = B.as_seq h st
 
 let frame_invariant _ _ _ _ = ()
 
+let invariant_loc_in_footprint _ _ = ()
+
 let vcache_create () =
   B.gcmalloc #(option record) HS.root None (U32.uint_to_t (UInt.max_int U16.n))
 
